AwsCryptographicMaterialProviders/dafny/AwsCryptographyKeyStore/src/AwsCryptographyKeyStoreOperations.dfy
@@ -131,14 +131,14 @@ module AwsCryptographyKeyStoreOperations refines AbstractAwsCryptographyKeyStore
       createInput := input;
     }
 
-    //= aws-encryption-sdk-specification/framework/branch-key-store.md#wrapped-branch-key-creation
+    //= aws-encryption-sdk-specification/framework/branch-key-store.md#branch-key-and-beacon-key-creation
     //# - `timestamp`: a timestamp for the current time.
     //# This timestamp MUST be in ISO8601 format in UTC, to microsecond precision (e.g. “YYYY-MM-DDTHH:mm:ss.ssssssZ“)
     var timestamp :- Time.GetCurrentTimeStamp()
     .MapFailure(e => Types.KeyStoreException(message := e));
 
     var maybeBranchKeyVersion := UUID.GenerateUUID();
-    //= aws-encryption-sdk-specification/framework/branch-key-store.md#wrapped-branch-key-creation
+    //= aws-encryption-sdk-specification/framework/branch-key-store.md#branch-key-and-beacon-key-creation
     //# - `version`: a new guid. This guid MUST be [version 4 UUID](https://www.ietf.org/rfc/rfc4122.txt)
     var branchKeyVersion :- maybeBranchKeyVersion
     .MapFailure(e => Types.KeyStoreException(message := e));
@@ -156,11 +156,11 @@ module AwsCryptographyKeyStoreOperations refines AbstractAwsCryptographyKeyStore
     );
   }
 
-  predicate VersionKeyEnsuresPublicly(input: VersionKeyInput, output: Result<(), Error>)
+  predicate VersionKeyEnsuresPublicly(input: VersionKeyInput, output: Result<VersionKeyOutput, Error>)
   {true}
 
   method VersionKey(config: InternalConfig, input: VersionKeyInput)
-    returns (output: Result<(), Error>)
+    returns (output: Result<VersionKeyOutput, Error>)
   {
     :- Need(0 < |input.branchKeyIdentifier|, Types.KeyStoreException(message := "Empty string not supported for identifier."));
 
