AwsCryptographicMaterialProviders/dafny/AwsCryptographyKeyStore/src/GetKeys.dfy
@@ -18,6 +18,7 @@ module GetKeys {
   import Types = AwsCryptographyKeyStoreTypes
   import DDB = ComAmazonawsDynamodbTypes
   import KMS = ComAmazonawsKmsTypes
+  import UTF8
 
   method GetActiveKeyAndUnwrap(
     input: Types.GetActiveBranchKeyInput,
@@ -29,12 +30,176 @@ module GetKeys {
     ddbClient: DDB.IDynamoDBClient
   )
     returns (output: Result<Types.GetActiveBranchKeyOutput, Types.Error>)
+    requires ddbClient.Modifies !! kmsClient.Modifies
+
     requires kmsClient.ValidState() && ddbClient.ValidState()
     modifies ddbClient.Modifies, kmsClient.Modifies
     ensures ddbClient.ValidState() && kmsClient.ValidState()
 
-    ensures output.Success? ==>
-              input.branchKeyIdentifier == output.value.branchKeyMaterials.branchKeyIdentifier
+    ensures
+      //= aws-encryption-sdk-specification/framework/branch-key-store.md#getactivebranchkey
+      //= type=implication
+      //# To get the active version for the branch key id from the keystore
+      //# this operation MUST call AWS DDB `GetItem`
+      //# using the `branch-key-id` as the Partition Key and `"branch:ACTIVE"` value as the Sort Key.
+      && |ddbClient.History.GetItem| == |old(ddbClient.History.GetItem)| + 1
+      && Seq.Last(ddbClient.History.GetItem).input.Key
+         == map[
+              Structure.BRANCH_KEY_IDENTIFIER_FIELD := DDB.AttributeValue.S(input.branchKeyIdentifier),
+              Structure.TYPE_FIELD := DDB.AttributeValue.S(Structure.BRANCH_KEY_ACTIVE_TYPE)
+            ]
+
+    ensures output.Success?
+            ==>
+
+              && Seq.Last(ddbClient.History.GetItem).output.Success?
+              && Seq.Last(ddbClient.History.GetItem).output.value.Item.Some?
+              && var activeItem := Seq.Last(ddbClient.History.GetItem).output.value.Item.value;
+
+              //= aws-encryption-sdk-specification/framework/branch-key-store.md#getactivebranchkey
+              //= type=implication
+              //# The AWS DDB response MUST contain the fields defined in the [branch keystore record format](#record-format).
+              && Structure.BranchKeyItem?(activeItem)
+              && activeItem[Structure.HIERARCHY_VERSION].N?
+              && Structure.BRANCH_KEY_ACTIVE_VERSION_FIELD in activeItem
+
+              && KMSKeystoreOperations.AttemptKmsOperation?(kmsConfiguration, Structure.ToBranchKeyContext(activeItem, logicalKeyStoreName))
+
+              //= aws-encryption-sdk-specification/framework/branch-key-store.md#getactivebranchkey
+              //= type=implication
+              //# The operation MUST decrypt the branch key according to the [AWS KMS Branch Key Decryption](#aws-kms-branch-key-decryption) section.
+
+              && var versionEncryptionContext := Structure.ToBranchKeyContext(activeItem, logicalKeyStoreName);
+
+              //= aws-encryption-sdk-specification/framework/branch-key-store.md#aws-kms-branch-key-decryption
+              //= type=implication
+              //# Every key in the constructed [encryption context](#encryption-context)
+              //# except `tableName`
+              //# MUST exist as a string attribute in the AWS DDB response item.
+              && versionEncryptionContext.Keys - {Structure.TABLE_FIELD} < activeItem.Keys
+
+              //= aws-encryption-sdk-specification/framework/branch-key-store.md#aws-kms-branch-key-decryption
+              //= type=implication
+              //# Every value in the constructed [encryption context](#encryption-context)
+              //# except the logical table name
+              //# MUST equal the value with the same key in the AWS DDB response item.
+              && (forall k <- versionEncryptionContext.Keys - {Structure.TABLE_FIELD}
+                    :: match k
+                       case HIERARCHY_VERSION => versionEncryptionContext[Structure.HIERARCHY_VERSION] == activeItem[Structure.HIERARCHY_VERSION].N
+                       case _ => versionEncryptionContext[k] == activeItem[k].S)
+
+              //= aws-encryption-sdk-specification/framework/branch-key-store.md#aws-kms-branch-key-decryption
+              //= type=implication
+              //# The key `enc` MUST NOT exist in the constructed [encryption context](#encryption-context).
+              && Structure.BRANCH_KEY_FIELD !in  versionEncryptionContext
+
+              //= aws-encryption-sdk-specification/framework/branch-key-store.md#aws-kms-branch-key-decryption
+              //= type=implication
+              //# The operation MUST use the configured `KMS SDK Client` to decrypt the value of the branch key field.
+              && |kmsClient.History.Decrypt| == |old(kmsClient.History.Decrypt)| + 1
+
+              //= aws-encryption-sdk-specification/framework/branch-key-store.md#aws-kms-branch-key-decryption
+              //= type=implication
+              //# When calling [AWS KMS Decrypt](https://docs.aws.amazon.com/kms/latest/APIReference/API_Decrypt.html),
+              //# the keystore operation MUST call with a request constructed as follows:
+              && var decryptRequest := Seq.Last(kmsClient.History.Decrypt).input;
+
+              //= aws-encryption-sdk-specification/framework/branch-key-store.md#aws-kms-branch-key-decryption
+              //= type=implication
+              //# - `KeyId` MUST be the configured `AWS KMS Key ARN` in the [AWS KMS Configuration](#aws-kms-configuration) for this keystore
+              && decryptRequest.KeyId == Some(kmsConfiguration.kmsKeyArn)
+
+              //= aws-encryption-sdk-specification/framework/branch-key-store.md#aws-kms-branch-key-decryption
+              //= type=implication
+              //# - `CiphertextBlob` MUST be the `enc` attribute value on the AWS DDB response item
+              && decryptRequest.CiphertextBlob == activeItem[Structure.BRANCH_KEY_FIELD].B
+
+              //= aws-encryption-sdk-specification/framework/branch-key-store.md#aws-kms-branch-key-decryption
+              //= type=implication
+              //# Every attribute except for `enc` on the AWS DDB response item
+              //# MUST be authenticated in the decryption of `enc`
+
+              //= aws-encryption-sdk-specification/framework/branch-key-store.md#aws-kms-branch-key-decryption
+              //= type=implication
+              //# - `EncryptionContext` MUST be the [encryption context](#encryption-context) constructed above
+              && decryptRequest.EncryptionContext == Some(versionEncryptionContext)
+
+              //= aws-encryption-sdk-specification/framework/branch-key-store.md#aws-kms-branch-key-decryption
+              //= type=implication
+              //# - `GrantTokens` MUST be this keystore's [grant tokens](https://docs.aws.amazon.com/kms/latest/developerguide/concepts.html#grant_token).
+              && decryptRequest.GrantTokens == Some(grantTokens)
+
+              && Seq.Last(kmsClient.History.Decrypt).output.Success?
+              && Seq.Last(kmsClient.History.Decrypt).output.value.Plaintext.Some?
+              && var decryptResponse := Seq.Last(kmsClient.History.Decrypt).output.value;
+
+
+              //= aws-encryption-sdk-specification/framework/branch-key-store.md#branch-key-materials-from-authenticated-encryption-context
+              //= type=implication
+              //# The `type` attribute MUST either be equal to `"branch:ACTIVE"` or start with `"version:"`.
+              && versionEncryptionContext[Structure.TYPE_FIELD] == Structure.BRANCH_KEY_ACTIVE_TYPE
+
+              //= aws-encryption-sdk-specification/framework/branch-key-store.md#branch-key-materials-from-authenticated-encryption-context
+              //= type=implication
+              //# If the `type` attribute is equal to `"branch:ACTIVE"`
+              //# then the authenticated encryption context MUST have a `version` attribute
+              //# and the version string is this value.
+              && Structure.BRANCH_KEY_ACTIVE_VERSION_FIELD in versionEncryptionContext
+              && var versionString := versionEncryptionContext[Structure.BRANCH_KEY_ACTIVE_VERSION_FIELD];
+              && UTF8.Encode(versionString[|Structure.BRANCH_KEY_TYPE_PREFIX|..]).Success?
+
+              //= aws-encryption-sdk-specification/framework/branch-key-store.md#branch-key-materials-from-authenticated-encryption-context
+              //= type=implication
+              //# If the `type` attribute start with `"version:"` then the version string MUST be equal to this value.
+              && !(Structure.BRANCH_KEY_TYPE_PREFIX < versionEncryptionContext[Structure.TYPE_FIELD])
+
+              //= aws-encryption-sdk-specification/framework/branch-key-store.md#getactivebranchkey
+              //= type=implication
+              //# This operation MUST return the constructed [branch key materials](./structures.md#branch-key-materials).
+              && output.value.branchKeyMaterials
+                 //= aws-encryption-sdk-specification/framework/branch-key-store.md#getactivebranchkey
+                 //= type=implication
+                 //# This GetActiveBranchKey MUST construct [beacon key materials](./structures.md#beacon-key-materials)
+                 //# according to [Branch Key Materials From Authenticated Encryption Context](#branch-key-materials-from-authenticated-encryption-context).
+                 == Types.BranchKeyMaterials(
+                      //= aws-encryption-sdk-specification/framework/branch-key-store.md#branch-key-materials-from-authenticated-encryption-context
+                      //= type=implication
+                      //# - [Branch Key](./structures.md#branch-key) MUST be the [decrypted branch key material](#aws-kms-branch-key-decryption)
+                      branchKey := decryptResponse.Plaintext.value,
+                      //= aws-encryption-sdk-specification/framework/branch-key-store.md#branch-key-materials-from-authenticated-encryption-context
+                      //= type=implication
+                      //# - [Branch Key Id](./structures.md#branch-key-id) MUST be the `branch-key-id`
+                      branchKeyIdentifier := versionEncryptionContext[Structure.BRANCH_KEY_IDENTIFIER_FIELD],
+
+                      //= aws-encryption-sdk-specification/framework/branch-key-store.md#branch-key-materials-from-authenticated-encryption-context
+                      //= type=implication
+                      //# - [Branch Key Version](./structures.md#branch-key-version)
+                      //# The version string MUST start with `branch:version:`.
+                      //# The remaining string encoded as UTF8 bytes MUST be the Branch Key version.
+                      branchKeyVersion := UTF8.Encode(versionString[|Structure.BRANCH_KEY_TYPE_PREFIX|..]).value,
+
+                      encryptionContext := map[]
+
+                    )
+
+              && output.value.branchKeyMaterials.branchKeyIdentifier == input.branchKeyIdentifier
+
+    ensures
+      //= aws-encryption-sdk-specification/framework/branch-key-store.md#getactivebranchkey
+      //= type=implication
+      //# If the record does not contain the defined fields, this operation MUST fail.
+      || (&& |ddbClient.History.GetItem| == |old(ddbClient.History.GetItem)| + 1
+          && Seq.Last(ddbClient.History.GetItem).output.Success?
+          && Seq.Last(ddbClient.History.GetItem).output.value.Item.Some?
+          && !Structure.ActiveBranchKeyItem?(Seq.Last(ddbClient.History.GetItem).output.value.Item.value)
+          ==> output.Failure?)
+
+      //= aws-encryption-sdk-specification/framework/branch-key-store.md#getactivebranchkey
+      //= type=implication
+      //# If the branch key fails to decrypt, GetActiveBranchKey MUST fail.
+      || (&& |kmsClient.History.Decrypt| == |old(kmsClient.History.Decrypt)| + 1
+          && Seq.Last(kmsClient.History.Decrypt).output.Failure?
+          ==> output.Failure?)
   {
 
     var branchKeyItem :- DDBKeystoreOperations.GetActiveBranchKeyItem(
@@ -79,12 +244,179 @@ module GetKeys {
     ddbClient: DDB.IDynamoDBClient
   )
     returns (output: Result<Types.GetBranchKeyVersionOutput, Types.Error>)
+    requires ddbClient.Modifies !! kmsClient.Modifies
+
     requires kmsClient.ValidState() && ddbClient.ValidState()
     modifies ddbClient.Modifies, kmsClient.Modifies
     ensures ddbClient.ValidState() && kmsClient.ValidState()
-    ensures output.Success? ==>
-              && input.branchKeyIdentifier == output.value.branchKeyMaterials.branchKeyIdentifier
-    // && TODO add version info
+
+
+
+    ensures
+      //= aws-encryption-sdk-specification/framework/branch-key-store.md#getbranchkeyversion
+      //= type=implication
+      //# To get a branch key from the keystore this operation MUST call AWS DDB `GetItem`
+      //# using the `branch-key-id` as the Partition Key and "version:" + `branchKeyVersion` value as the Sort Key.
+      && |ddbClient.History.GetItem| == |old(ddbClient.History.GetItem)| + 1
+      && Seq.Last(ddbClient.History.GetItem).input.Key
+         == map[
+              Structure.BRANCH_KEY_IDENTIFIER_FIELD := DDB.AttributeValue.S(input.branchKeyIdentifier),
+              Structure.TYPE_FIELD := DDB.AttributeValue.S(Structure.BRANCH_KEY_TYPE_PREFIX + input.branchKeyVersion)
+            ]
+
+    ensures output.Success?
+            ==>
+
+              && Seq.Last(ddbClient.History.GetItem).output.Success?
+              && Seq.Last(ddbClient.History.GetItem).output.value.Item.Some?
+              && var versionItem := Seq.Last(ddbClient.History.GetItem).output.value.Item.value;
+
+              //= aws-encryption-sdk-specification/framework/branch-key-store.md#getbranchkeyversion
+              //= type=implication
+              //# The AWS DDB response MUST contain the fields defined in the [branch keystore record format](#record-format).
+              && Structure.BranchKeyItem?(versionItem)
+              && versionItem[Structure.HIERARCHY_VERSION].N?
+              && Structure.BRANCH_KEY_ACTIVE_VERSION_FIELD !in versionItem
+              && Structure.BRANCH_KEY_TYPE_PREFIX < versionItem[Structure.TYPE_FIELD].S
+
+              && KMSKeystoreOperations.AttemptKmsOperation?(kmsConfiguration, Structure.ToBranchKeyContext(versionItem, logicalKeyStoreName))
+
+              //= aws-encryption-sdk-specification/framework/branch-key-store.md#getbranchkeyversion
+              //= type=implication
+              //# The operation MUST decrypt the branch key according to the [AWS KMS Branch Key Decryption](#aws-kms-branch-key-decryption) section.
+
+              && var versionEncryptionContext := Structure.ToBranchKeyContext(versionItem, logicalKeyStoreName);
+
+              //= aws-encryption-sdk-specification/framework/branch-key-store.md#aws-kms-branch-key-decryption
+              //= type=implication
+              //# Every key in the constructed [encryption context](#encryption-context)
+              //# except `tableName`
+              //# MUST exist as a string attribute in the AWS DDB response item.
+              && versionEncryptionContext.Keys - {Structure.TABLE_FIELD} < versionItem.Keys
+
+              //= aws-encryption-sdk-specification/framework/branch-key-store.md#aws-kms-branch-key-decryption
+              //= type=implication
+              //# Every value in the constructed [encryption context](#encryption-context)
+              //# except the logical table name
+              //# MUST equal the value with the same key in the AWS DDB response item.
+              && (forall k <- versionEncryptionContext.Keys - {Structure.TABLE_FIELD}
+                    :: match k
+                       case HIERARCHY_VERSION => versionEncryptionContext[Structure.HIERARCHY_VERSION] == versionItem[Structure.HIERARCHY_VERSION].N
+                       case _ => versionEncryptionContext[k] == versionItem[k].S)
+
+              //= aws-encryption-sdk-specification/framework/branch-key-store.md#aws-kms-branch-key-decryption
+              //= type=implication
+              //# The key `enc` MUST NOT exist in the constructed [encryption context](#encryption-context).
+              && Structure.BRANCH_KEY_FIELD !in  versionEncryptionContext
+
+              //= aws-encryption-sdk-specification/framework/branch-key-store.md#aws-kms-branch-key-decryption
+              //= type=implication
+              //# The operation MUST use the configured `KMS SDK Client` to decrypt the value of the branch key field.
+              && |kmsClient.History.Decrypt| == |old(kmsClient.History.Decrypt)| + 1
+
+              //= aws-encryption-sdk-specification/framework/branch-key-store.md#aws-kms-branch-key-decryption
+              //= type=implication
+              //# When calling [AWS KMS Decrypt](https://docs.aws.amazon.com/kms/latest/APIReference/API_Decrypt.html),
+              //# the keystore operation MUST call with a request constructed as follows:
+              && var decryptRequest := Seq.Last(kmsClient.History.Decrypt).input;
+
+              //= aws-encryption-sdk-specification/framework/branch-key-store.md#aws-kms-branch-key-decryption
+              //= type=implication
+              //# - `KeyId` MUST be the configured `AWS KMS Key ARN` in the [AWS KMS Configuration](#aws-kms-configuration) for this keystore
+              && decryptRequest.KeyId == Some(kmsConfiguration.kmsKeyArn)
+
+              //= aws-encryption-sdk-specification/framework/branch-key-store.md#aws-kms-branch-key-decryption
+              //= type=implication
+              //# - `CiphertextBlob` MUST be the `enc` attribute value on the AWS DDB response item
+              && decryptRequest.CiphertextBlob == versionItem[Structure.BRANCH_KEY_FIELD].B
+
+              //= aws-encryption-sdk-specification/framework/branch-key-store.md#aws-kms-branch-key-decryption
+              //= type=implication
+              //# Every attribute except for `enc` on the AWS DDB response item
+              //# MUST be authenticated in the decryption of `enc`
+
+              //= aws-encryption-sdk-specification/framework/branch-key-store.md#aws-kms-branch-key-decryption
+              //= type=implication
+              //# - `EncryptionContext` MUST be the [encryption context](#encryption-context) constructed above
+              && decryptRequest.EncryptionContext == Some(versionEncryptionContext)
+
+              //= aws-encryption-sdk-specification/framework/branch-key-store.md#aws-kms-branch-key-decryption
+              //= type=implication
+              //# - `GrantTokens` MUST be this keystore's [grant tokens](https://docs.aws.amazon.com/kms/latest/developerguide/concepts.html#grant_token).
+              && decryptRequest.GrantTokens == Some(grantTokens)
+
+              && Seq.Last(kmsClient.History.Decrypt).output.Success?
+              && Seq.Last(kmsClient.History.Decrypt).output.value.Plaintext.Some?
+              && var decryptResponse := Seq.Last(kmsClient.History.Decrypt).output.value;
+
+
+              //= aws-encryption-sdk-specification/framework/branch-key-store.md#branch-key-materials-from-authenticated-encryption-context
+              //= type=implication
+              //# The `type` attribute MUST either be equal to `"branch:ACTIVE"` or start with `"version:"`.
+              && Structure.BRANCH_KEY_TYPE_PREFIX < versionEncryptionContext[Structure.TYPE_FIELD]
+
+              //= aws-encryption-sdk-specification/framework/branch-key-store.md#branch-key-materials-from-authenticated-encryption-context
+              //= type=implication
+              //# If the `type` attribute start with `"version:"` then the version string MUST be equal to this value.
+              && Structure.BRANCH_KEY_TYPE_PREFIX < versionEncryptionContext[Structure.TYPE_FIELD]
+              && var versionString := versionEncryptionContext[Structure.TYPE_FIELD];
+              && UTF8.Encode(versionString[|Structure.BRANCH_KEY_TYPE_PREFIX|..]).Success?
+
+              //= aws-encryption-sdk-specification/framework/branch-key-store.md#branch-key-materials-from-authenticated-encryption-context
+              //= type=implication
+              //# If the `type` attribute is equal to `"branch:ACTIVE"`
+              //# then the authenticated encryption context MUST have a `version` attribute
+              //# and the version string is this value.
+              && Structure.BRANCH_KEY_ACTIVE_VERSION_FIELD !in versionEncryptionContext
+
+              //= aws-encryption-sdk-specification/framework/branch-key-store.md#getbranchkeyversion
+              //= type=implication
+              //# This operation MUST return the constructed [branch key materials](./structures.md#branch-key-materials).
+              && output.value.branchKeyMaterials
+                 //= aws-encryption-sdk-specification/framework/branch-key-store.md#getbranchkeyversion
+                 //= type=implication
+                 //# This GetBranchKeyVersion MUST construct [beacon key materials](./structures.md#beacon-key-materials)
+                 //# according to [Branch Key Materials From Authenticated Encryption Context](#branch-key-materials-from-authenticated-encryption-context).
+                 == Types.BranchKeyMaterials(
+                      //= aws-encryption-sdk-specification/framework/branch-key-store.md#branch-key-materials-from-authenticated-encryption-context
+                      //= type=implication
+                      //# - [Branch Key](./structures.md#branch-key) MUST be the [decrypted branch key material](#aws-kms-branch-key-decryption)
+                      branchKey := decryptResponse.Plaintext.value,
+                      //= aws-encryption-sdk-specification/framework/branch-key-store.md#branch-key-materials-from-authenticated-encryption-context
+                      //= type=implication
+                      //# - [Branch Key Id](./structures.md#branch-key-id) MUST be the `branch-key-id`
+                      branchKeyIdentifier := versionEncryptionContext[Structure.BRANCH_KEY_IDENTIFIER_FIELD],
+
+                      //= aws-encryption-sdk-specification/framework/branch-key-store.md#branch-key-materials-from-authenticated-encryption-context
+                      //= type=implication
+                      //# - [Branch Key Version](./structures.md#branch-key-version)
+                      //# The version string MUST start with `branch:version:`.
+                      //# The remaining string encoded as UTF8 bytes MUST be the Branch Key version.
+                      branchKeyVersion := UTF8.Encode(versionString[|Structure.BRANCH_KEY_TYPE_PREFIX|..]).value,
+
+                      encryptionContext := map[]
+
+                    )
+
+              && output.value.branchKeyMaterials.branchKeyIdentifier == input.branchKeyIdentifier
+
+
+    ensures
+      //= aws-encryption-sdk-specification/framework/branch-key-store.md#getbranchkeyversion
+      //= type=implication
+      //# If the record does not contain the defined fields, this operation MUST fail.
+      || (&& |ddbClient.History.GetItem| == |old(ddbClient.History.GetItem)| + 1
+          && Seq.Last(ddbClient.History.GetItem).output.Success?
+          && Seq.Last(ddbClient.History.GetItem).output.value.Item.Some?
+          && !Structure.VersionBranchKeyItem?(Seq.Last(ddbClient.History.GetItem).output.value.Item.value)
+          ==> output.Failure?)
+
+      //= aws-encryption-sdk-specification/framework/branch-key-store.md#getbranchkeyversion
+      //= type=implication
+      //# If the branch key fails to decrypt, this operation MUST fail.
+      || (&& |kmsClient.History.Decrypt| == |old(kmsClient.History.Decrypt)| + 1
+          && Seq.Last(kmsClient.History.Decrypt).output.Failure?
+          ==> output.Failure?)
   {
 
     var branchKeyItem :- DDBKeystoreOperations.GetVersionBranchKeyItem(
@@ -129,9 +461,12 @@ module GetKeys {
     ddbClient: DDB.IDynamoDBClient
   )
     returns (output: Result<Types.GetBeaconKeyOutput, Types.Error>)
+    requires ddbClient.Modifies !! kmsClient.Modifies
+
     requires kmsClient.ValidState() && ddbClient.ValidState()
     modifies ddbClient.Modifies, kmsClient.Modifies
     ensures ddbClient.ValidState() && kmsClient.ValidState()
+
     ensures output.Success? ==>
               && input.branchKeyIdentifier == output.value.beaconKeyMaterials.beaconKeyIdentifier
   {
